src/program_proof/single/election.v
@@ -1,0 +1,44 @@
+From iris.proofmode Require Import base tactics classes.
+From Perennial.base_logic Require Import lib.own.
+From iris.bi.lib Require Import fractional.
+From Perennial.program_proof Require Import proof_prelude.
+From Perennial.base_logic Require Export lib.ghost_map.
+From iris.algebra Require Import excl agree auth gmap csum.
+
+(* Library with resources and invariants to protect resources with an election *)
+Section election.
+
+Definition one_shotR V := csumR (exclR unitR) (agreeR (leibnizO V)).
+
+Class electionG Σ := PaxosG {
+  election_voteG :> inG Σ fracR;
+}.
+
+Context `{!electionG Σ}.
+Context `{!invG Σ}.
+
+Definition vote (n_pred:nat) (γ:gname) : iProp Σ :=
+  own γ (1/(pos_to_Qp (Pos.of_nat n_pred)))%Qp
+.
+
+Definition election_inv (P:iProp Σ) γ : iProp Σ :=
+  P
+  ∨
+  ∃ q, (own γ q%Qp) ∗ ⌜(1/2 < q)%Qp⌝
+.
+
+Definition N := nroot .@ "election".
+
+Definition is_election γ P : iProp Σ :=
+  inv N (election_inv P γ).
+
+Lemma claim_victory γ P (S:gset nat) n :
+  (2*size S) > (n+1) →
+  is_election γ P -∗
+  ([∗ set] k ∈ S, vote n γ) -∗
+  P
+.
+Proof.
+Admitted.
+
+End election.
